\documentclass[20pt]{extarticle}
\usepackage{amsmath}
\setlength{\oddsidemargin}{-2em}
\setlength{\evensidemargin}{-2em}
\addtolength{\textwidth}{4em}
\setlength{\topmargin}{-7em}
\addtolength{\textheight}{15em}
\pagestyle{empty}
\title{Error propagation of weighted average}
\author{Kei Ito}

\begin{document}

\begin{align}
    x_{1}, x_{2}, \hdots, x_{N}
\end{align}

\begin{align}
    \sigma_{x_{1}}^{2}, \sigma_{x_{2}}^{2}, \hdots, \sigma_{x_{N}}^{2}
\end{align}

\begin{align}
    u = \sum_{i=1}^{N}a_{i}x_{i}
\end{align}

\begin{align}
    u
    &= \left.\sum_{i=1}^{N}a_{i}x_{i} \middle/ \sum_{i=1}^{N}a_{i}\right.\\
    \label{eq:defA}
    &= \frac{1}{A}\sum_{i=1}^{N}a_{i}x_{i}
    \hspace{1em}\left(A = \sum_{i=1}^{N}a_{i}\right)
\end{align}

\begin{align}
    a_{i}
    &=\left(\sum_{i=1}^{N}\frac{1}{\sigma_{x_{i}}^{2}}\right)^{-1}\frac{1}{\sigma_{x_{i}}^{2}}\\
    \sigma_{u}^{2}
    &= \left(\sum_{i=1}^{N}\frac{1}{\sigma_{x_{i}}^{2}}\right)^{-1}
\end{align}

\begin{align}\label{eq:zero}
    \frac{\partial \sigma_{u}^{2}}{\partial a_{j}}=0
\end{align}

\begin{align}
    \sigma_{u}^{2}=\sum_{i=1}^{N}\left(\frac{\partial u}{\partial x_{i}}\right)^{2}\sigma_{x_{i}}^{2}
\end{align}

\begin{align}
    \label{eq:ai}
    \frac{\partial u}{\partial x_{i}}
    =\frac{\partial}{\partial x_{i}}\frac{1}{A}\sum_{j=1}^{N}a_{j}x_{j}
    =\frac{a_{i}}{A}
\end{align}

\begin{align}
    \sigma_{u}^{2}
    &\overset{(\ref{eq:ai})}{=}\sum_{i=1}^{N}\left(\frac{a_{i}}{A}\right)^{2}\sigma_{x_{i}}^{2}\\
    &=\frac{1}{A^{2}}\sum_{i=1}^{N}a_{i}^{2}\sigma_{x_{i}}^{2}\\
    \label{eq:defB}
    &=\frac{B}{A^{2}}
    \hspace{1em}\left(B = \sum_{i=1}^{N}a_{i}^{2}\sigma_{x_{i}}^{2}\right)
\end{align}

\begin{align}
    \frac{\partial}{\partial a_{j}}\frac{B}{A^{2}}&=0\\
    \left(\frac{\partial B}{\partial a_{j}}\right)\frac{1}{A^{2}}
    +B\left(\frac{\partial}{\partial a_{j}}\frac{1}{A^{2}}\right)&=0\\
    \frac{1}{A^{2}}\left(\frac{\partial B}{\partial a_{j}}\right)
    -\frac{2B}{A^{3}}\left(\frac{\partial A}{\partial a_{j}}\right)&=0
\end{align}

\begin{align}
    \frac{\partial A}{\partial a_{j}}
    =\frac{\partial}{\partial a_{j}}\sum_{i=1}^{N}a_{i}
    =1
\end{align}

\begin{align}
    \frac{\partial B}{\partial a_{j}}
    =\frac{\partial}{\partial a_{j}}\sum_{i=1}^{N}a_{i}^{2}\sigma_{x_{i}}^{2}
    =2a_{i}\sigma_{x_{i}}^{2}
\end{align}

\begin{align}
    \frac{2a_{j}\sigma_{x_{j}}^{2}}{A^{2}}
    -\frac{2B}{A^{3}}&=0\\
    a_{j}\sigma_{x_{j}}^{2}
    -\frac{B}{A}&=0\\
    \label{eq:aiwithAB}
    a_{j}
    &=\frac{B}{A}\frac{1}{\sigma_{x_{j}}^{2}}
\end{align}

\begin{align}
    \sum_{i=1}^{N}a_{i}
    &=\sum_{i=1}^{N}\frac{B}{A}\frac{1}{\sigma_{x_{i}}^{2}}\\
    A
    &=\frac{B}{A}\sum_{i=1}^{N}\frac{1}{\sigma_{x_{i}}^{2}}\\
    \label{eq:B}
    B
    &=A^{2}\left(\sum_{i=1}^{N}\frac{1}{\sigma_{x_{i}}^{2}}\right)^{-1}
\end{align}

\begin{align}
    \label{eq:normalizeA}
    A
    &\overset{(\ref{eq:defA})}{=}\sum_{i=1}^{N}a_{i}=1
\end{align}

\begin{align}
    \label{eq:resultB}
    B
    &\overset{(\ref{eq:B})}{=}A^{2}\left(\sum_{i=1}^{N}\frac{1}{\sigma_{x_{i}}^{2}}\right)^{-1}
    \overset{(\ref{eq:normalizeA})}{=}\left(\sum_{i=1}^{N}\frac{1}{\sigma_{x_{i}}^{2}}\right)^{-1}
\end{align}

\begin{align}
    \label{eq:resultA}
    a_{i}
    &\overset{(\ref{eq:aiwithAB})}{=}\frac{B}{A}\frac{1}{\sigma_{x_{i}}^{2}}
    \overset{(\ref{eq:normalizeA})}{=}B\frac{1}{\sigma_{x_{i}}^{2}}
    \overset{(\ref{eq:resultB})}{=}\left(\sum_{i=1}^{N}\frac{1}{\sigma_{x_{i}}^{2}}\right)^{-1}\frac{1}{\sigma_{x_{i}}^{2}}
\end{align}

\begin{align}
    \sigma_{u}^{2}
    &\overset{(\ref{eq:defB})}{=} \frac{B}{A^{2}}
    \overset{(\ref{eq:normalizeA})}{=} B
    \overset{(\ref{eq:resultB})}{=} \left(\sum_{i=1}^{N}\frac{1}{\sigma_{x_{i}}^{2}}\right)^{-1}
\end{align}

\end{document}
